Generated/erc20shim/ERC20Shim/Predicate.lean
@@ -25,6 +25,12 @@ def not_mem_private (a : Option UInt256) : Prop :=
   | some el => el ∉ ERC20Private.toFinset
   | none => true
 
+lemma not_mem_private_of_some {a : UInt256} (h : not_mem_private (some a)) :
+  a ∉ ERC20Private.toFinset := by
+  unfold not_mem_private at h
+  simp at h
+  exact h
+
 structure IsERC20 (erc20 : ERC20) (s : State) : Prop where
   hasSupply : s.evm.sload ERC20Private.totalSupply = erc20.supply
 
@@ -37,8 +43,8 @@ structure IsERC20 (erc20 : ERC20) (s : State) : Prop where
   hasAllowance :
     ∀ {owner spender}, (⟨owner, spender⟩ ∈ erc20.allowances) →
     ∃ (address  : UInt256) (intermediate : UInt256),
-    s.evm.keccak_map.lookup [ ↑owner , ERC20Private.allowances ] = some intermediate →
-    s.evm.keccak_map.lookup [ ↑spender , intermediate ] = some address →
+    s.evm.keccak_map.lookup [ ↑owner , ERC20Private.allowances ] = some intermediate ∧
+    s.evm.keccak_map.lookup [ ↑spender , intermediate ] = some address ∧
     erc20.allowances.lookup ⟨owner, spender⟩ = some (s.evm.sload address)
 
   storageDom :
@@ -48,14 +54,14 @@ structure IsERC20 (erc20 : ERC20) (s : State) : Prop where
         some address = s.evm.keccak_map.lookup [ ↑account, ERC20Private.balances ] }.toFinset ∪
       { address | ∃ owner spender,
         ⟨owner, spender⟩ ∈ erc20.allowances ∧
-        ∃ intermediate, s.evm.keccak_map.lookup [ ↑owner , ERC20Private.allowances ] = some intermediate ∧
+        ∀ {intermediate}, s.evm.keccak_map.lookup [ ↑owner , ERC20Private.allowances ] = some intermediate →
         s.evm.keccak_map.lookup [ ↑spender , intermediate ] = some address }.toFinset ∪
       ERC20Private.toFinset
 
   block_acc_range :
     ∀ {var},
-    not_mem_private (s.evm.keccak_map.lookup [ ↑var, ERC20Private.balances ]) ∧
-    not_mem_private (s.evm.keccak_map.lookup [ ↑var, ERC20Private.allowances ])
+    not_mem_private (s.evm.keccak_map.lookup [ var, ERC20Private.balances ]) ∧
+    not_mem_private (s.evm.keccak_map.lookup [ var, ERC20Private.allowances ])
 
   -- block_allowance_range :
   --   ∀ {owner}, s.evm.keccak_map.lookup [ ↑owner, ERC20Private.allowances ] ∉ ERC20Private.toFinset
